solutions/HTT_solutions.v
@@ -1,5 +1,409 @@
-Require Import ssreflect ssrbool ssrnat eqtype ssrfun.
+Add LoadPath "./../htt".
+Require Import ssreflect ssrbool ssrnat seq eqtype ssrfun.
+Require Import prelude pred pcm unionmap heap heaptac stmod stsep stlog stlogR.  
 
 Set Implicit Arguments.
 Unset Strict Implicit.
 Unset Printing Implicit Defensive.
+
+Definition llist (T : Type) := ptr.
+
+Section LList.
+Variable T : Type.
+Notation llist := (llist T).
+
+Fixpoint lseg (p q : ptr) (xs : seq T): Pred heap := 
+  if xs is x::xt then 
+    [Pred h | exists r h', 
+       h = p :-> x \+ (p .+ 1 :-> r \+ h') /\ h' \In lseg r q xt]
+  else [Pred h | p = q /\ h = Unit].
+
+Lemma lseg_null xs q h : 
+         valid h -> h \In lseg null q xs -> 
+         [/\ q = null, xs = [::] & h = Unit].
+Proof.
+case: xs=>[|x xs] D /= H; first by case: H=><- ->.
+case: H D=>r [h'][->] _. 
+by rewrite hvalidPtUn. 
+Qed. 
+
+Definition lseq p := lseg p null.
+
+Program Definition insert p x : 
+  {xs}, STsep (lseq p xs, [vfun y => lseq y (x::xs)]) :=
+  Do (q <-- allocb p 2; 
+      q ::= x;;
+      ret q). 
+Next Obligation. 
+apply: ghR=>i xs H _. 
+heval=>x1. 
+rewrite unitR -joinA. 
+heval. 
+Qed.
+
+Lemma lseq_null xs h : valid h -> h \In lseq null xs -> xs = [::] /\ h = Unit.
+Proof. by move=>D; case/(lseg_null D)=>_ ->. Qed.
+
+Lemma lseq_pos xs p h : 
+        p != null -> h \In lseq p xs -> 
+        exists x, exists r, exists h', 
+          [/\ xs = x :: behead xs, 
+              p :-> x \+ (p .+ 1 :-> r \+ h') = h & h' \In lseq r (behead xs)].
+Proof.
+case: xs=>[|x xs] /= H []. 
+ - move=>E. 
+   by rewrite E eq_refl in H.
+by move=>y [h'][->] H1; heval.
+Qed.
+
+Program Definition 
+remove p : {xs}, STsep (lseq p xs, [vfun y => lseq y (behead xs)]) :=
+  Do (if p == null then ret p 
+      else pnext <-- !(p .+ 1);
+           dealloc p;; 
+           dealloc p .+ 1;;
+           ret pnext). 
+
+Next Obligation.
+apply: ghR=>i xs H V; case: ifP H=>H1.
+- by rewrite (eqP H1); case/(lseq_null V)=>->->; heval. 
+case/(lseq_pos (negbT H1))=>x [q][h][->] <- /= H2.
+by heval; rewrite 2!unitL.
+Qed.
+
+End LList.
+
+(*******************************************************************)
+(**                     * Exercices *                              *)
+(*******************************************************************)
+
+(** 
+---------------------------------------------------------------------
+Exercise [Swapping two values]
+---------------------------------------------------------------------
+
+Implement in HTT a function that takes as arguments two pointers, [x]
+and [y], which point to natural numbers, and swaps their
+values. Reflect this effect in the function's specification and verify
+it.
+
+Hint: Instead of reading the value of a pointer into a variable [t]
+using the [t <-- !p] notation, you might need to specify the _type_ of
+the expected value explicitly by using the "de-sugared" version of the
+command [t <-- read T p], where [T] is the expected type. This way,
+the proof will be more straightforward.
+
+*)
+
+Program Definition swap (x y : ptr):
+  {(a b : nat)},
+  STsep (fun h => h = x :-> a \+ y :-> b,
+        [vfun (_: unit) h => h = x :-> b \+ y :-> a]) :=
+  Do (vx <-- read nat x;
+      vy <-- read nat y;
+      x ::= vy;;
+      y ::= vx).
+Next Obligation.
+apply:ghR=>_ [a b]->/= V.
+by heval.
+Qed.
+
+(**
+---------------------------------------------------------------------
+Exercise [Swapping two values without heval]
+---------------------------------------------------------------------
+
+Try to redo the previous exercise _without_ using the automation
+provided by the [heval] tactic. The goal of this exercise is to
+explore the library of HTT lemmas, mimicking the rules of the
+separation logic. You can alway displat the whole list of the
+available lemmas by running the command [Search _ (verify _ _ _)] and
+then refine the query for specific programs (e.g., [read] or [write]).
+*)
+
+Program Definition swap' (x y : ptr):
+  {(a b : nat)},
+  STsep (fun h => h = x :-> a \+ y :-> b,
+        [vfun (_: unit) h => h = x :-> b \+ y :-> a]) :=
+  Do (vx <-- read nat x;
+      vy <-- read nat y;
+      x ::= vy;;
+      y ::= vx).
+Next Obligation.
+apply:ghR=>_ [a b]->/= V.
+apply: bnd_seq; apply: val_read=>_.
+apply: bnd_seq; apply: val_readR =>/= _.
+apply: bnd_writeR=>/=.
+by apply val_writeR=>/=.
+Qed.
+
+
+(** 
+---------------------------------------------------------------------
+Exercise [Imperative procedure for Fibonacci numbers]
+---------------------------------------------------------------------
+
+The following program is an implementation in pseudocode of an
+efficient imperative implementation of the function [fib] that
+computes the [N]th Fibonacci number.  
+
+    fun fib (N : nat): nat = {
+      if N == 0 then ret 0
+       else if N == 1 then ret 1
+       else n <-- alloc 2;
+            x <-- alloc 1;
+            y <-- alloc 1;
+            res <-- 
+              (fix loop (_ : unit). 
+                 n' <-- !n;
+                 y' <-- !y;
+                 if n' == N then ret y'
+                 else tmp <-- !x;
+                      x ::= y';;
+                      x' <-- !x;
+                      y ::= x' + tmp;;
+                      n ::= n' + 1;;
+                      loop(tt))(tt).
+            dealloc n;;
+            dealloc x;;
+            dealloc y;;
+            ret res    
+    }
+
+Your task will be to prove its correctness with respect to the "pure"
+function [fib_pure] (which you should define in plain Coq) as well as
+the fact that it starts and ends in an empty heap.
+
+Hint: What is the loop invariant of the recursive computation defined
+by means of the [loop] function?
+
+Hint: Try to decompose the reasoning into verification of several code
+pieces as in the factorial example and then composing them together in
+the "main" function.
+
+*)
+
+Fixpoint fib_pure n := 
+  if n is n'.+1 then
+    if n' is n''.+1 then fib_pure n' + fib_pure n'' else 1
+  else 0.
+
+Definition fib_inv (n x y : ptr) (N : nat) h : Prop := 
+  exists n' x' y': nat, 
+  [/\ h = n :-> n'.+1 \+ x :-> x' \+ y :-> y',
+      x' = fib_pure n' & y' = fib_pure (n'.+1)].
+
+Definition fib_tp n x y N := 
+  unit ->
+     STsep (fib_inv n x y N, 
+           [vfun (res : nat) h => fib_inv n x y N h /\ res = fib_pure N]).
+
+Program Definition fib_acc (n x y : ptr) N: fib_tp n x y N := 
+  Fix (fun (loop : fib_tp n x y N) (_ : unit) => 
+    Do (n' <-- !n;
+        y' <-- !y;
+        if n' == N then ret y'
+        else tmp <-- !x;
+             x ::= y';;
+             x' <-- !x;
+             y ::= x' + tmp;;
+             n ::= n' + 1;;
+             loop tt)).
+
+Next Obligation.
+move=>h /=[n'][_][_][->{h}]->->.
+heval; case X: (n'.+1 == N)=>//.
+- by apply: val_ret=>_; move/eqP: X=><-/=.
+heval; apply: val_doR=>//. (* This line takes a while due to automation. *)
+move=>_.
+exists (n'.+1), (fib_pure (n'.+1)), (fib_pure n'.+1.+1).
+by rewrite addn1.
+Qed.
+
+Program Definition fib N : 
+  STsep ([Pred h | h = Unit], 
+         [vfun res h => res = fib_pure N /\ h = Unit]) := 
+  Do (
+   if N == 0 then ret 0
+   else if N == 1 then ret 1
+   else n   <-- alloc 2;
+        x <-- alloc 1;
+        y <-- alloc 1;
+        res <-- fib_acc n x y N tt;
+        dealloc n;;
+        dealloc x;;
+        dealloc y;;
+        ret res).
+
+Next Obligation.
+move=>_ /= ->.
+case N1: (N == 0)=>//; first by move/eqP: N1=>->; apply:val_ret. 
+case N2: (N == 1)=>//; first by move/eqP: N2=>->; apply:val_ret. 
+heval=>n; heval=>x; heval=>y; rewrite unitR joinC [x:->_ \+ _]joinC.
+apply: bnd_seq=>/=.
+apply: val_doR; last first=>//[res h|].
+- case; case=>n'[_][_][->{h}]->->->_.
+  by heval; rewrite !unitR.
+by exists 1, 1, 1.
+Qed.
+
+
+(** 
+---------------------------------------------------------------------
+Exercise [Value-returning list beheading]
+---------------------------------------------------------------------
+
+Define and verify function [remove_val] which is similar to remove,
+but also returns the value of the last "head" of the list before
+removal, in addition to the "next" pointer. Use Coq's [option] type to
+account for the possibility of an empty list in the result.
+
+*)
+
+Program Definition remove_val T p : {xs}, 
+  STsep (lseq p xs, 
+         [vfun y h => lseq y.1 (behead xs) h /\ 
+                      y.2 = (if xs is x::xs' then Some x else None)]) := 
+  Do (if p == null then ret (p, None) 
+      else x <-- read T p;
+           pnext <-- !(p .+ 1);
+           dealloc p;; 
+           dealloc p .+ 1;;
+           ret (pnext, Some x)). 
+Next Obligation.
+apply: ghR=>i xs H V; case: ifP H=>H1.
+- by rewrite (eqP H1); case/(lseq_null V)=>->->; heval. 
+case/(lseq_pos (negbT H1))=>x [q][h][->] <- /= H2.
+by heval; rewrite 2!unitL.
+Qed.
+
+(** 
+---------------------------------------------------------------------
+Exercise [Imperative in-place map]
+---------------------------------------------------------------------
+
+Define, specify and verify the imperative higher-order function
+[list_map] that takes arguments two types, [S] and [T], a pure
+function [f : T -> S] and a head [p] of a single-linked list,
+described by a predicate [lseq], and changes the list in place by
+applying [f] to each of its elements, while preserving the list's
+structure. The specification should reflect the fact that the new
+"logical" contents of the single-linked list are an [f] map-image of
+the old content.
+
+Hint: The lemmas [lseq_null] and [lseq_pos], proved previously, might
+be useful in the proof of the established specification.
+
+Hint: A tail-recursive call can be verified via HTT's [val_do] lemma,
+reminiscent to the rule %\Rule{App}%. However, the heap it operates
+with should be "massaged" appropriately via PCM's lemmas [joinC] and
+[joinA].
+
+Hint: A boolean lemma [negbT] can be useful to switch between
+different representations of inequality.
+
+*)
+
+Definition mapT T S (f : T -> S) : Type := 
+  forall p, {xs}, STsep (@lseq T p xs, 
+                         [vfun y h => y = tt /\ @lseq S p (map f xs) h]).
+
+Program Definition list_map T S p (f : T -> S) :
+   {xs}, STsep (@lseq T p xs, 
+                [vfun y h => y = tt /\ @lseq S p (map f xs) h]) :=
+    Fix (fun (loop : mapT f) (p : ptr) =>      
+      Do (if p == null 
+          then ret tt 
+          else x <-- read T p;
+               next <-- (read ptr p .+ 1);
+               p ::= f x;;
+               loop next)) p.
+Next Obligation.
+apply: ghR=>h xs H V. 
+case X: (p0 == null).
+- apply: val_ret=>_ /=;  split=>//. 
+  by move/eqP: X H=>-> /=; case/(lseq_null V)=>->->. 
+case/negbT /lseq_pos /(_ H): X=>x[next][h'][Z1] Z2 H1; subst h.
+heval.
+move/validR: V=> V1; apply: (gh_ex (behead xs)).
+rewrite [_ \+ h']joinC joinC -joinA; apply: val_do=>//=.
+case=>m[_]H2 V2; split=>//.
+rewrite [_ \+ p0 :-> _]joinC joinC. 
+by rewrite Z1 /=; exists next, m; rewrite joinA.
+Qed.
+
+
+(**
+---------------------------------------------------------------------
+Exercise [In-place list reversal]
+---------------------------------------------------------------------
+
+Let us define the following auxiliary predicates, where [shape_rev]
+splits the heap into two disjoint linked lists (by means of the
+separating conjunction [#]).
+
+*)
+
+Definition shape_rev T p s := [Pred h | h \In @lseq T p.1 s.1 # @lseq T p.2 s.2].
+
+(** 
+
+Then the in-place list reversal is implemented by means of the
+recursive function [reverse] with a loop invariant expressed using the
+type [revT].
+
+*)
+
+Definition revT T : Type := 
+  forall p, {ps}, STsep (@shape_rev T p ps, [vfun y => lseq y (rev ps.1 ++ ps.2)]).
+
+Program Definition 
+reverse T p : {xs}, STsep (@lseq T p xs, [vfun y => lseq y (rev xs)]) :=
+  Do (let: reverse := Fix (fun (reverse : revT T) p => 
+                        Do (if p.1 == null then ret p.2 
+                            else xnext <-- !p.1 .+ 1;
+                                 p.1 .+ 1 ::= p.2;;
+                                 reverse (xnext, p.1)))
+      in reverse (p, null)).
+
+(** 
+
+You're invited to conduct the verification of [reverse], proving
+that it satisfies the given specification.
+
+Hint: It might be a good idea to make use of the previously proved
+lemmas [lseq_null] and [lseq_pos].
+
+Hint: Be careful with the logical values of variables passed to the
+[gh_ex] lemma before verifying a recursive call of [reverse].
+
+Hint: A verification goal to a function defined via [Fix] can be
+reduced via the [val_doR] lemma or similar ones.
+
+Hint: The [shape_rev] predicate is in fact an existential in disguise:
+it can be proved by providing appropriate witnesses.
+
+Hint: Lemmas [rev_cons], [cat_rcons] and [cats0] from the [seq]
+library will be useful for establishing equalities between lists.
+
+*)
+
+Next Obligation.
+apply:ghR=>i[xs1 xs2]; case=>h1[h2][->{i}]/=[H1 H2] V1.
+case X: (p0 == null) H1=>H1.
+- apply: val_ret=>/=_; move/eqP: X=>X; subst p0.
+  move/validL: (V1)=>V3; case:(lseq_null V3 H1)=>Z1 Z2; subst xs1 h1=>/=.
+  by rewrite unitL. 
+case/negbT /(lseq_pos) /(_ H1): X=>x[next][h'][Exs]Z H3; subst h1.
+heval; rewrite -!joinA -!(joinCA h'); apply: (gh_ex (behead xs1, x::xs2)).
+apply: val_doR=>//=[V2|].
+ - exists h', (p0 :-> x \+ (p0 .+ 1 :-> p1 \+ h2)); split=>//; split=>//.
+   by exists p1, h2; rewrite !joinA.
+by move=> z m H4 _; rewrite Exs rev_cons cat_rcons.
+Qed.
+
+Next Obligation.
+apply: ghR=>i xs H V /=; apply: (gh_ex (xs, [::])).
+apply: val_doR=>//=[_|]; first by exists i, Unit; rewrite unitR. 
+by rewrite cats0.
+Qed.
